\documentclass[a4paper]{article}

%% Language and font encodings
\usepackage[english]{babel}
\usepackage[utf8x]{inputenc}
\usepackage[T1]{fontenc}

%% Sets page size and margins
\usepackage[a4paper,top=3cm,bottom=2cm,left=3cm,right=3cm,marginparwidth=1.75cm]{geometry}

%% Useful packages
\usepackage{amsmath}
\usepackage{graphicx}
\usepackage[colorinlistoftodos]{todonotes}
\usepackage[colorlinks=true, allcolors=blue]{hyperref}
\usepackage{float}
\usepackage{enumerate}
\usepackage{subfig}
\setlength\parindent{0pt}
\usepackage{amssymb}
\setcounter{section}{-1}
\title{MA 3475 Exam 1 Review Problems}

\begin{document}
\maketitle
Find the extremal(s) of the following functionals.

\section*{Problem 1}
$$J[y] = \int_a^b \left(3x + \sqrt{y'(x)}\right) \; dx $$

\begin{align*}
F(x,y,y') &= 3x + \sqrt{y'} \\
F_y &= 0, \quad F_{y'} = \frac{1}{2\sqrt{y'}} \\
0 &= F_y - \frac{d}{dx}F_{y'} = 0 - \frac{d}{dx}\left[\frac{1}{2\sqrt{y'}}\right] \quad \text{(Euler-Lagrange)} \\
\implies c &= \frac{1}{2\sqrt{y'}} \\
y'(x) &= 4c^2 =: c_1  \\
y(x) &= \int_a^b y'(x) \; dx = c_1x + c_2
\end{align*}

The constants $c_1,c_2$ can be determined if we know $y(a),y(b)$.
\section*{Problem 2}

$$J[y] = \int_a^b \left(y(x) - y(x)y'(x) + x(y'(x))^2\right) \; dx,\quad a > 0 $$

\begin{align*}
F(x,y,y') &= y-yy' + x(y')^2 \\
F_y &= 1-y', \quad F_{y'} = -y + 2xy' \\
0 &= F_y - \frac{d}{dx}F_{y'} = 1-y - \frac{d}{dx}\left[2xy' - y\right] \quad \text{(Euler-Lagrange)}\\
0&= 1-y' -2y' - 2xy'' + y' \\
0&= (-2x)y'' -2y' + 1 \\
y'' + \frac{1}{x}y &= \frac{1}{2x} \\
\mu(x) &= \exp\left(\int \frac{1}{x} \; dx \right) = x \\
xy'' + y &= \frac{1}{2} \\
\frac{d}{dx}\left[xy'\right] &= \frac{1}{2}\\
xy'(x) &= \frac{1}{2}x + c_1 \\
y'(x) &= \frac{1}{2} + \frac{c_1}{x} \\
y(x) &= \int_a^b y'(x) \; dx = \frac{1}{2}x + c_1\ln(x) + c_2
\end{align*}

The constants $c_1,c_2$ can be determined if we know $y(a),y(b)$.

\section*{Problem 3}

$$J[y] = \int_a^b \sqrt{1+(y'(x))^2} \; dx $$

\begin{align*}
F(x,y,y') &= F(y') = \sqrt{1 + (y')^2}\\
0 &= F_y - \frac{d}{dx}F_{y'} = 0 - \frac{d}{dx}\left[\frac{y'}{\sqrt{1+(y')^2}}\right] \quad \text{(Euler-Lagrange)} \\
\implies c &= \frac{y'}{\sqrt{1+(y')^2}}\\
y'(x) &= \frac{c}{\sqrt{1-c^2}} \\
y(x) &= \frac{c}{\sqrt{1-c^2}}x + c_2 \\
y(x) &= c_1x + c_2, \quad \left(c_1 = \frac{c}{\sqrt{1-c^2}} \right)\;.
\end{align*}

The constants $c_1,c_2$ can be determined if we know $y(a),y(b)$.

\section*{Problem 4}

$$J[y] = \int_a^b \left[2y(x) + (y'(x))^2\right] \; dx $$

\begin{align*}
F(x,y,y') &= F(y,y') = 2y + (y')^2\\
0 &= F_y - \frac{d}{dx}F_{y'} = 2 - \frac{d}{dx}\left[2y'\right] \quad \text{(Euler-Lagrange)} \\
\implies y''(x) &= 1 \\
y'(x) &= x + c_1 \\
y(x) &= \frac{x^2}{2} + c_1x + c_2
\end{align*}

The constants $c_1,c_2$ can be determined if we know $y(a),y(b)$.\\

We could also have used Beltrami's identity since $F(x,y,y') = F(y,y')$. 

\section*{Problem 5}

$$J[y] = \int_a^b \left[y^2(x) -4y(x)y'(x) + 4(y'(x)^2)\right] \; dx $$

\begin{align*}
F(x,y,y') &= F(y,y') = y^2 - 4yy' + 4(y')^2\\
0 &= F_y - \frac{d}{dx}F_{y'} = 2y - 4y' - \frac{d}{dx}\left[ -4y + 8y'\right] \quad \text{(Euler-Lagrange)} \\
0&= 2y-4y' +4y' -8y''\\
0&= 4y'' - y \\
\implies y(x) &= c_1e^{\frac{x}{2}} + c_2e^{-\frac{x}{2}} \quad (\text{using the characteristic equation method with } 4r^2 - 1 = 0)\\
\end{align*}
An alternative way to write this solution:

\begin{align*}
y(x) &= c_1e^{\frac{x}{2}} + c_2e^{-\frac{x}{2}} \\
&= (c_1+c_2)\frac{e^{x/2} + e^{-x/2}}{2} + (c_1 - c_2)\frac{e^{x/2} - e^{-x/2}}{2} \\
&= (c_1+c_2)\cosh(x/2) + (c_1-c_2)\sinh(x/2) \\
&= c_3\cosh(x/2) + c_4 \sinh(x/2) \;.
\end{align*}

As before, we need to know $y(a),y(b)$ in order to determine the constant coefficients. 



\end{document}